src/Specific/GF1305.v
@@ -15,6 +15,7 @@ Local Open Scope Z.
 
 Definition modulus : Z := 2^130 - 5.
 Lemma prime_modulus : prime modulus. Admitted.
+Definition int_width := 32%Z.
 
 Instance params1305 : PseudoMersenneBaseParams modulus.
   construct_params prime_modulus 5%nat 130.
@@ -26,16 +27,22 @@ Instance subCoeff : SubtractionCoefficient modulus params1305.
   apply Build_SubtractionCoefficient with (coeff := mul2modulus); cbv; auto.
 Defined.
 
+Definition freezePreconditions1305 : freezePreconditions params1305 int_width.
+Proof.
+  constructor; compute_preconditions.
+Defined.
+
 (* END PseudoMersenneBaseParams instance construction. *)
 
 (* Precompute k and c *)
 Definition k_ := Eval compute in k.
 Definition c_ := Eval compute in c.
+Definition c_subst : c = c_ := eq_refl c_.
 
 (* Makes Qed not take forever *)
 Opaque Z.shiftr Pos.iter Z.div2 Pos.div2 Pos.div2_up Pos.succ Z.land
   Z.of_N Pos.land N.ldiff Pos.pred_N Pos.pred_double Z.opp Z.mul Pos.mul
-  Let_In digits Z.add Pos.add Z.pos_sub.
+  Let_In digits Z.add Pos.add Z.pos_sub andb Z.eqb Z.ltb.
 
 Local Open Scope nat_scope.
 Lemma GF1305Base26_mul_reduce_formula :
@@ -45,8 +52,9 @@ Lemma GF1305Base26_mul_reduce_formula :
                       -> rep ls (f*g)%F}.
 Proof.
   eexists; intros ? ? Hf Hg.
-  pose proof (carry_mul_opt_rep k_ c_ (eq_refl k) (eq_refl c_) _ _ _ _ Hf Hg) as Hfg.
+  pose proof (carry_mul_opt_rep k_ c_ (eq_refl k) c_subst _ _ _ _ Hf Hg) as Hfg.
   compute_formula.
+  exact Hfg.
 Defined.
 
 Lemma GF1305Base26_add_formula :
@@ -58,17 +66,30 @@ Proof.
   eexists; intros ? ? Hf Hg.
   pose proof (add_opt_rep _ _ _ _ Hf Hg) as Hfg.
   compute_formula.
+  exact Hfg.
 Defined.
 
-Lemma GF25519Base25Point5_sub_formula :
-  forall f0 f1 f2 f3 f4 f5 f6 f7 f8 f9
-    g0 g1 g2 g3 g4 g5 g6 g7 g8 g9,
-    {ls | forall f g, rep [f0;f1;f2;f3;f4;f5;f6;f7;f8;f9] f
-                   -> rep [g0;g1;g2;g3;g4;g5;g6;g7;g8;g9] g
+Lemma GF1305Base26_sub_formula :
+  forall f0 f1 f2 f3 f4 g0 g1 g2 g3 g4,
+    {ls | forall f g, rep [f0;f1;f2;f3;f4] f
+                   -> rep [g0;g1;g2;g3;g4] g
                    -> rep ls (f - g)%F}.
 Proof.
   eexists.
   intros f g Hf Hg.
   pose proof (sub_opt_rep _ _ _ _ Hf Hg) as Hfg.
   compute_formula.
+  exact Hfg.
+Defined.
+
+Lemma GF1305Base26_freeze_formula :
+  forall f0 f1 f2 f3 f4,
+    {ls | forall x, rep [f0;f1;f2;f3;f4] x
+                 -> rep ls x}.
+Proof.
+  eexists.
+  intros x Hf.
+  pose proof (freeze_opt_preserves_rep _ c_subst freezePreconditions1305 _ _ Hf) as Hfreeze_rep.
+  compute_formula.
+  exact Hfreeze_rep.
 Defined.
